8–î–µ–Ω—å : 2024-08-18 
–í—Ä–µ–º—è : 14-23

Status : #Math  


# Appropriate links
[[]]

---

# üìèTheme : Theorem of Vieta


```ad-important

This in another way of solving quadratic equations that world only when the coefficient a equals to 1
```


 - According to this theorem 

 $$x^{2}+px+q=0$$
$$x_{1}+x_{2}=-p$$
$$x_{1}*x_{2}=q$$

### Where this formulas came from

$$(x-x_{1})(x-x_{2})=x^{2}-x_{1}x_{2}-x_{2}x+x_{1}$$
$$x^{2} -(x_{1}+x_{2})x +x_{1}x_{2}$$

$$x^{2}+px+q$$
$$p=-(x_{1}+x_{2}) \implies x_{1}+x_{2}=-p$$
$$q=x_{1}x_{2} $$

--- 

The idea of two roots in quadratic equation:
![[Pasted image 20240818160848.png]]

---

## 7 main situations in theorem of Vieta related equations

Example of the equation:
$$x^{2}-3x-4=0$$



1) $$x_{1}+x_{2}=3$$
2) $$x_{1}x_{2}=-4$$
3) $$\frac{1}{x_{1}}+\frac{1}{x_{2}}\implies\frac{{x_{2}+x_{1}}}{x_{1}x_{2}} =-\frac{3}{4}$$
4) $$x_{1}^{2}+x_{2}^{2}\implies(x_{1}+x_{2})^{2}-2x_{1}x_{2} \implies 3^{2}-2(-4)= 17$$
5) $$\frac{1}{x_{1}^{2}}+\frac{1}{x_{2}^{2}}\implies\frac{x_{1}^{2}+x_{2}^{2}}{x_{1}^{2}x_{2}^{2}}\implies\frac{(x_{1}+x_{2})^{2}-2x_{1}x_{2}}{x_{1}^{2}x_{2}^{2}}\implies\frac{9+8}{(-4)^{2}}=\frac{17}{16}$$
6) $$x_{1}^{3}+x_{2}^{3}=(x_{1}+x_{2})(x_{1}^{2}-x_{1}x_{2}+x_{2}^{2})=(x_{1}+x_{2})((x_{1}+x_{2})^{2}-3x_{1}x_{2})= 3((3)^{2}-3(-4))=63$$
7) $$x_{1}^{4}+x_{2}^{4}\implies(x_{1}^{2})^{2}+(x_{2}^{2})^{2}\implies(x_{1}^{2}+x_{2}^{2})^{2}-2(x_{1}^{2}x_{2}^{2})\implies((x_{1}+x_{2})^{2}-2x_{1}x_{2})^{2}-2(x_{1}^{2}x_{2}^{2}))\implies(9+8)^{2}-2(-4)^{2}=289-32=257$$


## For x with exponent 3


$$ax^{3}+bx^{2}+cx+d=0$$
$$x^{3}+\frac{b}{a}x^{2}+\frac{c}{a}x+\frac{d}{a}=0$$

----

$$x^{3}+px^{2}+qx+r=0$$

$$x_{1}+x_{2}+x_{3}=-p$$
$$x_{1}x_{2}+x_{2}x_{3}+x_{1}x_{3}=q$$
$$x_{1}x_{2}x_{3} =-r$$

![[Pasted image 20240829181047.png]]

---

